src/Preservation.v
@@ -27,6 +27,14 @@ Proof.
     subst; 
     eauto with local_hints).
   - inversion H_type_e2; subst. eauto with local_hints.
+  - apply T_Rec.
+    inversion H_step; subst.
+    assert (Maps.same_bindings (x |-> e'0; m) (x |-> e; m)).
+    {
+      apply Maps.same_bindings_update.
+      apply Maps.same_bindings_refl.
+    }
+    eapply Maps.same_bindings_trans; eauto.
 Qed.
 
 Theorem preservation' : ∀ e e' t,
@@ -38,5 +46,14 @@ Proof.
   try (inversion H_type; subst; 
     inversion H_step; subst;
     eauto with local_hints).
-    inversion H4. eauto with local_hints.
+    - inversion H4. eauto with local_hints.
+    - apply T_Rec.
+      inversion H_step; subst.
+      assert (Maps.same_bindings (x |-> e'0; fields) fields).
+      {
+        eapply Maps.same_bindings_shadow_add.
+        - apply Maps.same_bindings_refl.
+        - apply H5. 
+      }
+      eapply Maps.same_bindings_trans; eauto.
 Qed.
